cfrontend/SemanticsProofs.v
@@ -1,0 +1,20 @@
+Require Import Coqlib Errors Maps.
+Require Import Integers Floats Values AST Memory Allocator Builtins Events Globalenvs Tags.
+Require Import Ctypes Cop Csyntax Csem.
+Require Import Smallstep.
+Require Import List. Import ListNotations.
+Require Import String.
+
+Module PolicyInsensitivity (Ptr: Pointer) (Pol1: Policy) (Pol2: Policy)
+       (M: Memory Ptr) (A: Allocator Ptr).
+  Module M1 := M Pol1.
+  Module M2 := M Pol2.
+  Module A1 := A Pol1 M1.
+  Module A2 := A Pol2 M2.
+  Module Csem1 := Csem Ptr Pol1 M1 A1.
+  Import Csem1.
+  Module Csem2 := Csem Ptr Pol2 M2 A2.
+  Import Csem2.
+
+  Variable prog1 : Csem1.Csyntax.program.
+  Variable prog2 : Csem2.Csyntax.program.
