common/Tags.v
@@ -6,6 +6,8 @@ Require Import Values.
 Require Import Ctypes.
 Require Import Cabs.
 Require Import String.
+Require Import Builtins.
+Require Import Switch.
 
 Require Import List. Import ListNotations. (* list notations is a module inside list *)
 
@@ -96,8 +98,10 @@ Module Type Policy. (* anaaktge this is the interface for rules
   
 End Policy.
 
-Module TagLib (P:Policy).
-  Export P.
+Module TagLib (Ptr: Pointer) (Pol: Policy).
+  Export Pol.
+  Module Switch := Switch Ptr.
+  Export Switch.
   Export Values.
 
   Definition atom : Type := val * tag.
@@ -124,6 +128,7 @@ Module TagLib (P:Policy).
     apply Int64.eq_dec.
     apply Float.eq_dec.
     apply Float32.eq_dec.
+    apply Ptr.ptr_eq_dec.
     decide equality.
     repeat decide equality.
     repeat decide equality.
